-

main/SortingFun.v
@@ -11,6 +11,7 @@ Require Export SortingFun_common.
 Require Export SortingFun_isort.
 Require Export SortingFun_ssort.
 Require Export SortingFun_bsort.
+Require Export SortingFun_msort.
 
 Theorem fold_sorted : ∀ A f (l : list A), (is_sorted f l = true) = sorted f l.
 Proof. easy. Qed.
@@ -137,49 +138,6 @@ f_equal.
 now apply IHla.
 Qed.
 
-(* merge sort *)
-
-Fixpoint merge_loop {A} (rel : A → A → bool) it la lb :=
-  match it with
-  | 0 => []
-  | S it' =>
-      match la, lb with
-      | [], _ => lb
-      | _, [] => la
-      | a :: la', b :: lb' =>
-          if rel a b then a :: merge_loop rel it' la' lb
-          else b :: merge_loop rel it' la lb'
-      end
-  end.
-
-Definition merge {A} (rel : A → A → bool) la lb :=
-  merge_loop rel (length la + length lb) la lb.
-
-Fixpoint split_list {A} (la : list A) :=
-  match la with
-  | [] | [_] => (la, [])
-  | a :: b :: lb =>
-      let (l1, l2) := split_list lb in
-      (a :: l1, b :: l2)
-  end.
-
-Fixpoint msort_loop {A} (rel : A → A → bool) it la :=
-  match it with
-  | 0 => la
-  | S it' =>
-      let (l1, l2) := split_list la in
-      let l3 := msort_loop rel it' l1 in
-      let l4 := msort_loop rel it' l2 in
-      merge rel l3 l4
-  end.
-
-Definition msort {A} (rel : A → _) la :=
-  msort_loop rel (length la) la.
-
-Theorem fold_merge : ∀ A (rel : A → _) la lb,
-  merge_loop rel (length la + length lb) la lb = merge rel la lb.
-Proof. easy. Qed.
-
 (* *)
 
 Theorem split_list_nil_l : ∀ A (la lb : list A),
@@ -234,138 +192,6 @@ cbn.
 rewrite (IHla lb); [ easy | ].
 cbn in Hlen.
 now destruct Hlen as [H| H]; [ left | right ]; now apply Nat.succ_inj in H.
-Qed.
-
-Theorem merge_loop_length : ∀ A (rel : A → _) la lb it,
-  length (la ++ lb) ≤ it
-  → length (merge_loop rel it la lb) = length (la ++ lb).
-Proof.
-intros * Hit.
-revert la lb Hit.
-induction it; intros; cbn. {
-  apply Nat.le_0_r, List.length_zero_iff_nil in Hit.
-  now rewrite Hit.
-}
-destruct la as [| a]; [ easy | ].
-destruct lb as [| b]; [ now cbn; rewrite List.app_nil_r | ].
-remember (rel a b) as ab eqn:Hab; symmetry in Hab.
-destruct ab; cbn; f_equal. {
-  apply IHit; cbn in Hit.
-  now apply Nat.succ_le_mono in Hit.
-}
-rewrite IHit; cbn. {
-  do 2 rewrite List.length_app; cbn.
-  symmetry; apply Nat.add_succ_r.
-} {
-  rewrite List.length_app in Hit; cbn in Hit.
-  apply Nat.succ_le_mono in Hit.
-  now rewrite Nat.add_succ_r, <- List.length_app in Hit.
-}
-Qed.
-
-Theorem merge_length : ∀ A (rel : A → _) la lb,
-  length (merge rel la lb) = length (la ++ lb).
-Proof.
-intros.
-unfold merge.
-apply merge_loop_length.
-now rewrite List.length_app.
-Qed.
-
-Theorem split_list_length : ∀ A la (lb lc : list A),
-  split_list la = (lb, lc)
-  → length la = length lb + length lc.
-Proof.
-intros * Hs.
-remember (length la) as len eqn:Hlen; symmetry in Hlen |-*.
-revert la lb lc Hs Hlen.
-induction len as (len, IHlen) using lt_wf_rec; intros.
-destruct la as [| a]. {
-  now injection Hs; clear Hs; intros; subst lb lc.
-}
-destruct la as [| b]. {
-  now injection Hs; clear Hs; intros; subst lb lc.
-}
-cbn in Hs, Hlen.
-remember (split_list la) as ll eqn:Hll; symmetry in Hll.
-destruct ll as (ld, le).
-injection Hs; clear Hs; intros; subst lb lc.
-destruct len; [ easy | ].
-destruct len; [ easy | cbn ].
-rewrite Nat.add_succ_r; f_equal; f_equal.
-do 2 apply Nat.succ_inj in Hlen.
-apply (IHlen len) in Hll; [ easy | | easy ].
-now transitivity (S len).
-Qed.
-
-Theorem split_list_lengths : ∀ A (l la lb : list A),
-  split_list l = (la, lb)
-  → length la = length lb ∨ length la = S (length lb).
-Proof.
-intros * Hll.
-remember (length l) as len eqn:Hlen.
-revert l la lb Hlen Hll.
-induction len as (len, IHlen) using lt_wf_rec; intros.
-destruct l as [| a]; intros; cbn. {
-  now injection Hll; intros; subst la lb; left.
-}
-destruct l as [| b]; intros; cbn. {
-  now injection Hll; intros; subst la lb; right.
-}
-cbn in Hll.
-remember (split_list l) as ll eqn:H; symmetry in H.
-destruct ll as (lc, ld).
-injection Hll; clear Hll; intros; subst la lb.
-rename lc into la; rename ld into lb; rename H into Hll.
-destruct len; [ easy | ].
-destruct len; [ easy | ].
-cbn in Hlen |-*.
-do 2 apply Nat.succ_inj in Hlen.
-specialize (IHlen len) as H1.
-assert (H : len < S (S len)) by now transitivity (S len).
-specialize (H1 H); clear H.
-specialize (H1 l la lb Hlen Hll).
-now destruct H1 as [H1| H1]; rewrite H1; [ left | right ].
-Qed.
-
-Theorem msort_loop_length : ∀ A (rel : A → _) it la,
-  length (msort_loop rel it la) = length la.
-Proof.
-intros.
-revert la.
-induction it; intros; [ easy | cbn ].
-remember (split_list la) as ll eqn:Hll; symmetry in Hll.
-destruct ll as (lb, lc).
-rewrite merge_length.
-rewrite List.length_app.
-do 2 rewrite IHit.
-now symmetry; apply split_list_length.
-Qed.
-
-Theorem msort_loop_nil : ∀ A (rel : A → _) it,
-  msort_loop rel it [] = [].
-Proof.
-intros.
-induction it; [ easy | cbn ].
-now rewrite IHit; cbn.
-Qed.
-
-Theorem msort_loop_unit : ∀ A (rel : A → _) it a,
-  msort_loop rel it [a] = [a].
-Proof.
-intros.
-induction it; [ easy | cbn ].
-now rewrite IHit, msort_loop_nil.
-Qed.
-
-Theorem msort_loop_pair : ∀ A (rel : A → _) it a b,
-  rel a b = true
-  → msort_loop rel it [a; b] = [a; b].
-Proof.
-intros * Hab.
-induction it; [ easy | cbn ].
-do 2 rewrite msort_loop_unit; cbn.
-now rewrite Hab.
 Qed.
 
 Theorem split_list_cons_cons : ∀ A (l la lb : list A) a b,
@@ -619,6 +445,10 @@ destruct ca. {
   now rewrite Haa.
 }
 Qed.
+
+(*
+...
+*)
 
 Theorem sorted_merge_loop_cons_cons_r : ∀ A (rel : A → _),
   antisymmetric rel →
@@ -1661,15 +1491,6 @@ Qed.
 
 (* main *)
 
-Theorem bsort_when_sorted : ∀ A (rel : A → _),
-  ∀ l,
-  sorted rel l
-  → bsort rel l = l.
-Proof.
-intros * Hs.
-now apply bsort_loop_when_sorted.
-Qed.
-
 Theorem msort_when_sorted : ∀ A (rel : A → _),
   antisymmetric rel →
   transitive rel →
@@ -1685,14 +1506,6 @@ Qed.
 
 (* *)
 
-Theorem sorted_bsort : ∀ [A] {rel : A → _},
-  total_relation rel →
-  ∀ l, sorted rel (bsort rel l).
-Proof.
-intros * Htot *.
-now apply sorted_bsort_loop.
-Qed.
-
 Theorem sorted_msort : ∀ [A] {rel : A → _},
   total_relation rel →
   ∀ l, sorted rel (msort rel l).
@@ -1702,18 +1515,6 @@ now apply sorted_msort_loop.
 Qed.
 
 (* *)
-
-Theorem sorted_bsort_iff : ∀ A (rel : A → A → bool),
-  total_relation rel →
-  ∀ l, sorted rel l ↔ bsort rel l = l.
-Proof.
-intros * Htot *.
-split; [ now apply bsort_when_sorted | ].
-intros Hs.
-specialize sorted_bsort as H1.
-specialize (H1 _ rel Htot l).
-now rewrite Hs in H1.
-Qed.
 
 Theorem sorted_msort_iff : ∀ A (rel : A → A → bool),
   antisymmetric rel →
@@ -1731,13 +1532,6 @@ Qed.
 
 (* *)
 
-Theorem permuted_bsort : ∀ {A} {eqb : A → _} rel (Heqb : equality eqb),
-  ∀ l, permutation eqb l (bsort rel l).
-Proof.
-intros.
-now apply permuted_bsort_loop.
-Qed.
-
 Theorem permuted_msort : ∀ {A} {eqb : A → _} rel (Heqb : equality eqb),
   ∀ l, permutation eqb l (msort rel l).
 Proof.
@@ -1746,28 +1540,6 @@ now apply permuted_msort_loop.
 Qed.
 
 (* *)
-
-Theorem bsort_when_permuted : ∀ A (eqb rel : A → _),
-  equality eqb →
-  antisymmetric rel →
-  transitive rel →
-  total_relation rel →
-  ∀ la lb,
-  permutation eqb la lb
-  → bsort rel la = bsort rel lb.
-Proof.
-intros * Heqb Hant Htra Htot * Hpab.
-specialize (sorted_bsort Htot la) as Hsa.
-specialize (sorted_bsort Htot lb) as Hsb.
-specialize (permuted_bsort rel Heqb la) as Hpa.
-specialize (permuted_bsort rel Heqb lb) as Hpb.
-assert (Hsab : permutation eqb (bsort rel la) (bsort rel lb)). {
-  eapply (permutation_trans Heqb); [ | apply Hpb ].
-  eapply (permutation_trans Heqb); [ | apply Hpab ].
-  now apply (permutation_sym Heqb).
-}
-now apply (sorted_sorted_permuted Heqb Hant Htra).
-Qed.
 
 Theorem msort_when_permuted : ∀ A (eqb rel : A → _),
   equality eqb →
