main/SortingFun_msort.v
@@ -1,0 +1,182 @@
+(* merge sort *)
+
+Set Nested Proofs Allowed.
+
+Require Import Utf8 Arith.
+Import List.ListNotations.
+
+Require Import Misc PermutationFun.
+Require Import SortingFun_common.
+
+Fixpoint merge_loop {A} (rel : A → A → bool) it la lb :=
+  match it with
+  | 0 => []
+  | S it' =>
+      match la, lb with
+      | [], _ => lb
+      | _, [] => la
+      | a :: la', b :: lb' =>
+          if rel a b then a :: merge_loop rel it' la' lb
+          else b :: merge_loop rel it' la lb'
+      end
+  end.
+
+Definition merge {A} (rel : A → A → bool) la lb :=
+  merge_loop rel (length la + length lb) la lb.
+
+Fixpoint split_list {A} (la : list A) :=
+  match la with
+  | [] | [_] => (la, [])
+  | a :: b :: lb =>
+      let (l1, l2) := split_list lb in
+      (a :: l1, b :: l2)
+  end.
+
+Fixpoint msort_loop {A} (rel : A → A → bool) it la :=
+  match it with
+  | 0 => la
+  | S it' =>
+      let (l1, l2) := split_list la in
+      let l3 := msort_loop rel it' l1 in
+      let l4 := msort_loop rel it' l2 in
+      merge rel l3 l4
+  end.
+
+Definition msort {A} (rel : A → _) la :=
+  msort_loop rel (length la) la.
+
+Theorem fold_merge : ∀ A (rel : A → _) la lb,
+  merge_loop rel (length la + length lb) la lb = merge rel la lb.
+Proof. easy. Qed.
+
+Theorem merge_loop_length : ∀ A (rel : A → _) la lb it,
+  length (la ++ lb) ≤ it
+  → length (merge_loop rel it la lb) = length (la ++ lb).
+Proof.
+intros * Hit.
+revert la lb Hit.
+induction it; intros; cbn. {
+  apply Nat.le_0_r, List.length_zero_iff_nil in Hit.
+  now rewrite Hit.
+}
+destruct la as [| a]; [ easy | ].
+destruct lb as [| b]; [ now cbn; rewrite List.app_nil_r | ].
+remember (rel a b) as ab eqn:Hab; symmetry in Hab.
+destruct ab; cbn; f_equal. {
+  apply IHit; cbn in Hit.
+  now apply Nat.succ_le_mono in Hit.
+}
+rewrite IHit; cbn. {
+  do 2 rewrite List.length_app; cbn.
+  symmetry; apply Nat.add_succ_r.
+} {
+  rewrite List.length_app in Hit; cbn in Hit.
+  apply Nat.succ_le_mono in Hit.
+  now rewrite Nat.add_succ_r, <- List.length_app in Hit.
+}
+Qed.
+
+Theorem merge_length : ∀ A (rel : A → _) la lb,
+  length (merge rel la lb) = length (la ++ lb).
+Proof.
+intros.
+unfold merge.
+apply merge_loop_length.
+now rewrite List.length_app.
+Qed.
+
+Theorem split_list_length : ∀ A la (lb lc : list A),
+  split_list la = (lb, lc)
+  → length la = length lb + length lc.
+Proof.
+intros * Hs.
+remember (length la) as len eqn:Hlen; symmetry in Hlen |-*.
+revert la lb lc Hs Hlen.
+induction len as (len, IHlen) using lt_wf_rec; intros.
+destruct la as [| a]. {
+  now injection Hs; clear Hs; intros; subst lb lc.
+}
+destruct la as [| b]. {
+  now injection Hs; clear Hs; intros; subst lb lc.
+}
+cbn in Hs, Hlen.
+remember (split_list la) as ll eqn:Hll; symmetry in Hll.
+destruct ll as (ld, le).
+injection Hs; clear Hs; intros; subst lb lc.
+destruct len; [ easy | ].
+destruct len; [ easy | cbn ].
+rewrite Nat.add_succ_r; f_equal; f_equal.
+do 2 apply Nat.succ_inj in Hlen.
+apply (IHlen len) in Hll; [ easy | | easy ].
+now transitivity (S len).
+Qed.
+
+Theorem msort_loop_length : ∀ A (rel : A → _) it la,
+  length (msort_loop rel it la) = length la.
+Proof.
+intros.
+revert la.
+induction it; intros; [ easy | cbn ].
+remember (split_list la) as ll eqn:Hll; symmetry in Hll.
+destruct ll as (lb, lc).
+rewrite merge_length.
+rewrite List.length_app.
+do 2 rewrite IHit.
+now symmetry; apply split_list_length.
+Qed.
+
+Theorem msort_loop_nil : ∀ A (rel : A → _) it,
+  msort_loop rel it [] = [].
+Proof.
+intros.
+induction it; [ easy | cbn ].
+now rewrite IHit; cbn.
+Qed.
+
+Theorem msort_loop_unit : ∀ A (rel : A → _) it a,
+  msort_loop rel it [a] = [a].
+Proof.
+intros.
+induction it; [ easy | cbn ].
+now rewrite IHit, msort_loop_nil.
+Qed.
+
+Theorem msort_loop_pair : ∀ A (rel : A → _) it a b,
+  rel a b = true
+  → msort_loop rel it [a; b] = [a; b].
+Proof.
+intros * Hab.
+induction it; [ easy | cbn ].
+do 2 rewrite msort_loop_unit; cbn.
+now rewrite Hab.
+Qed.
+
+Theorem split_list_lengths : ∀ A (l la lb : list A),
+  split_list l = (la, lb)
+  → length la = length lb ∨ length la = S (length lb).
+Proof.
+intros * Hll.
+remember (length l) as len eqn:Hlen.
+revert l la lb Hlen Hll.
+induction len as (len, IHlen) using lt_wf_rec; intros.
+destruct l as [| a]; intros; cbn. {
+  now injection Hll; intros; subst la lb; left.
+}
+destruct l as [| b]; intros; cbn. {
+  now injection Hll; intros; subst la lb; right.
+}
+cbn in Hll.
+remember (split_list l) as ll eqn:H; symmetry in H.
+destruct ll as (lc, ld).
+injection Hll; clear Hll; intros; subst la lb.
+rename lc into la; rename ld into lb; rename H into Hll.
+destruct len; [ easy | ].
+destruct len; [ easy | ].
+cbn in Hlen |-*.
+do 2 apply Nat.succ_inj in Hlen.
+specialize (IHlen len) as H1.
+assert (H : len < S (S len)) by now transitivity (S len).
+specialize (H1 H); clear H.
+specialize (H1 l la lb Hlen Hll).
+now destruct H1 as [H1| H1]; rewrite H1; [ left | right ].
+Qed.
